\section*{Aufgabe 1)}
\subsection*{a)}
Mit $s = 0$ ergibt sich für $b_0$:
\begin{align*}
	\frac{\partial}{\partial b_0} \ln[L(b_0,0)] &= \frac{N_\text{off}}{b_0} + \frac{N_\text{on}}{b_0} - (1+\alpha) = 0 \\
	b_0 &= \frac{N_\text{off} + N_\text{on}}{1+\alpha}
\end{align*}

Der Fehler $\sigma_{b_0}^2$ wird über berechnet:
\begin{align*}
	\sigma_{b_0}^2 &= \frac{\partial^2 \ln(L)}{\partial b_0^2} = -\frac{N_\text{off} + N_\text{on}}{b_0^2}	\\
	&= -\frac{N_\text{off} + N_\text{on}} {\left(\frac{N_\text{off} + N_\text{on}}{1+\alpha}\right)^2}	= -\frac{(1 + \alpha)^2}{N_\text{off} + N_\text{on}}
\end{align*}



\subsection*{b)}
\begin{align*}
	\lambda &= \frac{L_0}{\hat{L}} = e^{\ln\left(\frac{L_0}{\hat{L}}\right)} =
	e^{\ln(L_0) - \ln(\hat{L})}	\\
	&= \exp[N_\text{off} \ln(b_0) + N_\text{on} \ln(\alpha b_0) - (1+\alpha)b_0 - \ln(N_\text{off}!) - \ln(N_\text{on}!)	\\
	& \;\;-(N_\text{off} \ln(\hat{b}) + N_\text{on} \ln(\hat{s}+\alpha\hat{b}) - (1+\alpha)\hat{b} - \hat{s} - \ln(N_\text{off}!) - \ln(N_\text{on}!) )]	\\
	&= e^{N_\text{off} \ln(b_0)}\; e^{N_\text{on} \ln(\alpha b_0)}\; e^{-(1+\alpha)b_0}\; e^{-N_\text{off} \ln{\hat{b}}}\; e^{-N_\text{on} \ln(\hat{s}+ \alpha\hat{b})}\; e^{(1+\alpha)\hat{b}}\; e^{\hat{s}}	\\
	&= b_0^{N_\text{off}}\; b_0^{N_\text{on}}\; \alpha^{N_\text{on}}\; \hat{b}^{-N_\text{off}}\; (\hat{s}+\alpha\hat{b})^{-N_\text{on}}\; e^{-(1+\alpha)b_0}\; e^{(1+\alpha)\hat{b}} \; e^{\hat{s}}	\\
	&=\frac{(N_\text{on}+N_\text{off})^{N_\text{on}+N_\text{off}}}{(1+\alpha)^{N_\text{off}+N_\text{on}}}\; \alpha^{N_\text{on}}\; N_\text{off}^{-N_\text{off}}\; N_\text{on}^{-N_\text{on}}\; e^{N_\text{off} + N_\text{on}}\; e^{(1+\alpha)N_\text{off}}\; e^{N_\text{on} - \alpha{N_\text{off}}}
\end{align*}
